pk_dh_game.v
@@ -6,7 +6,7 @@ From iris.algebra Require Import numbers.
 From iris.heap_lang Require Import notation proofmode adequacy.
 From iris.heap_lang.lib Require Import par.
 From cryptis Require Import lib term cryptis primitives tactics.
-From cryptis Require Import session nsl dh nsl_dh.
+From cryptis Require Import role nown session pk_auth dh pk_dh.
 
 Set Implicit Arguments.
 Unset Strict Implicit.
@@ -37,8 +37,8 @@ Definition game : val := λ: "mkchan",
   let: "pkR'" := recv "c" in
   bind: "kt" := is_key "pkR'" in
   assert: ("kt" = repr Enc) in
-  let: "res" := nsl_dh_init N "c" Spec.zero "skI" "pkI" "pkR'" |||
-                nsl_dh_resp N "c" Spec.zero "skR" "pkR" in
+  let: "res" := pk_dh_init N "c" "skI" "pkI" "pkR'" |||
+                pk_dh_resp N "c" "skR" "pkR" in
   bind: "sesskI" := Fst "res" in
   bind: "resR" := Snd "res" in
   let: "pkI'" := Fst "resR" in
@@ -55,16 +55,17 @@ Lemma wp_game (mkchan : val) :
   {{{ True }}} mkchan #() {{{ v, RET v; channel v }}} -∗
   enc_pred_token ⊤ -∗
   key_pred_token ⊤ -∗
+  nown_token session_name ⊤ -∗
   WP game mkchan {{ v, ⌜v = NONEV ∨ v = SOMEV #true⌝ }}.
 Proof.
-iIntros "wp_mkchan enc_tok key_tok"; rewrite /game; wp_pures.
-pose (P rl (t1 t2 t3 t4 : term) :=
-  (∃ k, ⌜(if rl is Init then t3 else t4) =
+iIntros "wp_mkchan enc_tok key_tok nown_tok"; rewrite /game; wp_pures.
+pose (P rl (kI kR kS : term) :=
+  (∃ k, ⌜(if rl is Init then kI else kR) =
          Spec.tag (nroot.@"key") k⌝ ∧
-        nonce_meta k (nroot.@"nsl") (t1, t2, t3, t4))%I).
-iMod (nsl_dh_alloc N P Spec.zero with "enc_tok") as (γdh) "#ctx" => //.
+        nonce_meta k (nroot.@"nsl") (kI, kR, kS))%I).
+iMod (pk_dh_alloc N P with "nown_tok enc_tok") as "[#ctx _]" => //.
 iMod (key_pred_set (nroot.@"key") (λ kt _, ⌜kt = Enc⌝)%I with "key_tok")
-  as "#?" => //.
+  as "[#? _]" => //.
 wp_bind (mkchan _); iApply "wp_mkchan" => //.
 iIntros "!> %c #cP".
 wp_pures; wp_bind (mknonce _).
@@ -100,28 +101,29 @@ case: kt epkR' ekt => // -> _.
 iApply (wp_par (λ v, ∃ a : option term, ⌜v = repr a⌝ ∗ _)%I
                (λ v, ∃ a : option (term * term), ⌜v = repr a⌝ ∗ _)%I
           with "[init] [resp]").
-- iApply (wp_nsl_dh_init P P with "[//] [//] [] [] [//] [init]") => //.
-  + by rewrite sterm_TInt.
+- iApply (wp_pk_dh_init with "[//] [//] [] [] [init]") => //.
   + rewrite [pterm (TKey Enc (Spec.tag _ _))]pterm_TKey sterm_tag.
     iRight; iSplit => //.
     iExists _, _, _; eauto.
-  + iIntros (ga gb).
-    iMod (term_meta_set _ _ (ga, gb, Spec.tag (nroot.@"key") kI, kR')
-                        (nroot.@"nsl") with "init"); first by solve_ndisj.
-    by iModIntro; iSplit; iExists _; iSplit; eauto.
-  + iIntros (a) "H"; iExists a; iSplit; first done.
+  + iIntros "%nI %nR".
+    set (kS := mk_session_key _ _ _).
+    set (kI' := Spec.tag _ _).
+    iMod (term_meta_set _ _ (kI', kR', kS) (nroot.@"nsl") with "init").
+      solve_ndisj.
+    iModIntro. iExists _. by iFrame.
+  + iIntros "!> %a H". iExists a. iSplit; first done.
     iApply "H".
-- iApply (wp_nsl_dh_resp P P with "[//] [//] [] [] [resp]") => //.
-  + eauto.
-  + by rewrite sterm_TInt.
+- iApply (wp_pk_dh_resp with "[//] [//] [] [resp]") => //.
   + rewrite [pterm (TKey Enc (Spec.tag _ _))]pterm_TKey sterm_tag.
     iRight; iSplit => //.
     iExists _, _, _; eauto.
-  + iIntros (ga gb kI').
-    iMod (term_meta_set _ _ (ga, gb, kI', Spec.tag (nroot.@"key") kR)
-                        (nroot.@"nsl") with "resp"); first by solve_ndisj.
-    by iModIntro; iSplit; iExists _; iSplit; eauto.
-  + iIntros (a) "H"; iExists a; iSplit; first done.
+  + iIntros "%kI' %nI %nR".
+    set (kS := mk_session_key _ _ _).
+    set (kR'' := Spec.tag _ _).
+    iMod (term_meta_set _ _ (kI', kR'', kS) (nroot.@"nsl") with "resp").
+      solve_ndisj.
+    iModIntro. iExists _. by iFrame.
+  + iIntros "!> %a H"; iExists a; iSplit; first done.
     iApply "H".
 iIntros (v1 v2) "[H1 H2]".
 iDestruct "H1" as (a) "[-> H1]".
@@ -129,8 +131,8 @@ iDestruct "H2" as (b) "[-> H2]".
 iModIntro; wp_pures.
 case: a => [gabI|]; wp_pures; last by eauto.
 case: b => [[pkI' gabR]|]; wp_pures; last by eauto.
-iDestruct "H1" as (a gb) "#(-> & s_gabI & init & H1)".
-iDestruct "H2" as (kI' b ga) "#(-> & -> & p_pkI' & s_gabR & resp & H2)".
+iDestruct "H1" as "(#s_gabI & #confI & H1)".
+iDestruct "H2" as (kI') "(-> & #p_pkI' & #gabR & #confR & H2)".
 iAssert ((nonce_meta kI (nroot.@"pub") () → False) ∧
          |==> nonce_meta kI (nroot.@"pub") ())%I with "[pub]" as "pub"; first iSplit.
 - iIntros "#contra".
@@ -138,7 +140,7 @@ iAssert ((nonce_meta kI (nroot.@"pub") () → False) ∧
 - by iApply (term_meta_set with "pub"); eauto.
 wp_eq_term e_pkR; wp_pures.
   case: e_pkR => <- {kR'}.
-  iDestruct "H1" as "[[contra|contra]|H1]".
+  iDestruct "H1" as "[#[contra|contra]|H1]".
   - rewrite [pterm (TKey Dec _)]pterm_TKey pterm_tag.
     iDestruct "contra" as "[contra|[_ contra]]".
       iSpecialize ("p_kI" with "contra").
@@ -159,13 +161,14 @@ wp_eq_term e_pkR; wp_pures.
   wp_pures; wp_bind (send _ _); iApply wp_send => //.
     rewrite [pterm skR]pterm_TKey pterm_tag; iModIntro.
     iLeft; iApply "p_kR"; eauto.
-  iDestruct "H1" as (b') "# (-> & resp' & sec)".
-  iDestruct "resp" as (k) "[%resp resp]".
-  case/Spec.tag_inj: resp => [_ <- {k}].
-  iDestruct "resp'" as (k) "[%resp resp']".
-  case/Spec.tag_inj: resp => [_ <- {k}].
-  iPoseProof (term_meta_agree with "resp resp'") as "%valid".
-  case: valid => -> /TExp_inj [_ /(Permutation_singleton_inj b b') <-] ->.
+  iDestruct "H1" as "(#p_gabI & token & #sess)".
+  iPoseProof (session_key_confirmation _ Resp with "sess") as "confR'".
+  iDestruct "confR" as (k) "[%conf confR]".
+  case/Spec.tag_inj: conf => [_ <- {k}].
+  iDestruct "confR'" as (k) "[%conf confR']".
+  case/Spec.tag_inj: conf => [_ <- {k}] /=.
+  iPoseProof (term_meta_agree with "confR confR'") as "%valid".
+  case: valid => -> -> {kI' gabR}.
   wp_pures.
   wp_bind (recv _); iApply wp_recv => //; iIntros (m) "#p_m".
   wp_pures; wp_bind (eq_term _ _); iApply wp_eq_term.
@@ -173,21 +176,21 @@ wp_eq_term e_pkR; wp_pures.
   wp_pures; wp_bind (eq_term _ _); iApply wp_eq_term.
   rewrite bool_decide_decide decide_True //.
   wp_pures; wp_bind (eq_term _ _); iApply wp_eq_term.
-  rewrite !Spec.texpA TExpC2 bool_decide_decide decide_True //.
-  case: (decide (m = TExp Spec.zero [b; a])) => [->|ne].
-    by iDestruct ("sec" with "p_m") as ">[]".
+  rewrite bool_decide_decide decide_True //.
+  case: (decide (m = gabI)) => [->|ne].
+    by iDestruct ("p_gabI" with "p_m") as ">[]".
   wp_pures; wp_bind (eq_term _ _); iApply wp_eq_term.
   rewrite bool_decide_decide decide_False //.
   wp_pures; eauto.
 wp_eq_term e_pkI; wp_pures; last by eauto.
 case: e_pkI => <- {kI'}.
-iDestruct "H2" as "[[contra|contra]|H2]".
+iDestruct "H2" as "[[#contra|#contra]|H2]".
 - rewrite [pterm (TKey Dec _)]pterm_TKey pterm_tag.
   iDestruct "contra" as "[contra|[_ contra]]".
     iSpecialize ("p_kI" with "contra").
     iAssert (▷ False)%I with "[pub]" as ">[]".
     iModIntro.
-    by iDestruct "pub" as "[pub _]"; iApply "pub"; eauto.
+    iDestruct "pub" as "[pub _]"; iApply "pub"; eauto.
   by iMod (wf_key_elim with "contra [//]") as "%".
 - rewrite [pterm (TKey Dec _)]pterm_TKey pterm_tag.
   iDestruct "contra" as "[contra|[_ contra]]".
@@ -195,13 +198,14 @@ iDestruct "H2" as "[[contra|contra]|H2]".
     iAssert (▷ False)%I with "[pub]" as ">[]".
     by iDestruct "pub" as "[pub _]"; iApply "pub"; eauto.
   by iMod (wf_key_elim with "contra [//]") as "%".
-iDestruct "H2" as (a') "#(-> & init' & ?)".
-iDestruct "init" as (k) "[%init init]".
-case/Spec.tag_inj: init => [_ <- {k}].
-iDestruct "init'" as (k) "[%init init']".
-case/Spec.tag_inj: init => [_ <- {k}].
-iPoseProof (term_meta_agree with "init init'") as "%valid".
-by case: valid e_pkR => _ _ -> /(_ eq_refl) [].
+iDestruct "H2" as "(#p_gabR & token & #H2)".
+iPoseProof (session_key_confirmation _ Init with "H2") as "confI'".
+iDestruct "confI" as (k) "[%conf confI]".
+case/Spec.tag_inj: conf => [_ <- {k}].
+iDestruct "confI'" as (k) "[%conf confI']".
+case/Spec.tag_inj: conf => [_ <- {k}].
+iPoseProof (term_meta_agree with "confI confI'") as "%valid".
+by case: valid e_pkR => -> _ /(_ eq_refl) [].
 Qed.
 
 End Game.
@@ -209,7 +213,7 @@ End Game.
 Definition F : gFunctors :=
   #[heapΣ; spawnΣ; cryptisΣ; sessionΣ].
 
-Lemma nsl_dh_secure (mkchan : val) σ₁ σ₂ (v : val) ts :
+Lemma pk_dh_secure (mkchan : val) σ₁ σ₂ (v : val) ts :
   (∀ `{!heapGS Σ, !cryptisG Σ},
      ⊢ {{{ True }}} mkchan #() {{{ c, RET c; channel c}}}) →
   rtc erased_step ([game mkchan], σ₁) (Val v :: ts, σ₂) →
@@ -221,6 +225,7 @@ apply (adequate_result NotStuck _ _ (λ v _, v = NONEV ∨ v = SOMEV #true)).
 apply: heap_adequacy.
 iIntros (?) "?".
 iMod (cryptisG_alloc _) as (?) "(enc_tok & key_tok & _)".
+iMod (sessionG_alloc _) as (?) "nown_tok".
 iApply (wp_game with "[] [enc_tok] [key_tok]") => //.
 iApply wp_mkchan.
 Qed.
